permutation proofs

proof/amd64/avx2/Keccak1600_avx2x4.ec
@@ -11,15 +11,17 @@ require import AllCore List Real Int IntDiv StdOrder.
 
 from Jasmin require import JModel_x86.
 
-from CryptoSpecs require import Bindings.
 from CryptoSpecs require export FIPS202_SHA3 FIPS202_Keccakf1600.
 from CryptoSpecs require import Keccakf1600_Spec Keccak1600_Spec FIPS202_SHA3_Spec.
+
+require import Keccak_bindings.
+require import Avx2_extra.
 
 from JazzEC require import Keccak1600_Jazz.
 
 
-from JazzEC require import WArray200.
-from JazzEC require import Array25 Array24 Array5.
+from JazzEC require import WArray200 WArray800.
+from JazzEC require import Array100 Array25.
 
 import IntOrder.
 
@@ -44,169 +46,13 @@ rewrite nth_iota; split; first smt().
 move=> _; rewrite ltzE; smt(leq_div2r).
 qed.
 
-require import Avx2_extra.
 
-import BitEncoding BitChunking.
-
-from JazzEC require import WArray800.
-
-op sliceget64_256_25 (arr: W256.t Array25.t) (offset: int) : W64.t = 
- if 8 %| offset
- then WArray800.get64_direct (WArray800.init256 (fun i => arr.[i])) (offset %/ 8)
- else W64.bits2w (take 64 (drop offset (flatten (map W256.w2bits (to_list arr))))).
-
-(*
-bind op [W256.t & W64.t & Array25.t] sliceget64_256_25 "asliceget".
-realize bvaslicegetP.
-move => /= arr offset; rewrite /sliceget64_256_25 /= => H k kb. 
-case (8 %| offset) => /= *; last by smt(W64.get_bits2w).
-rewrite /get64_direct pack8E initiE 1:/# /= initiE 1:/# /= initiE 1:/# /= bits8E initiE 1:/# /=.
-rewrite nth_take 1,2:/# nth_drop 1,2:/#.
-rewrite (BitEncoding.BitChunking.nth_flatten false 256 _). 
- by rewrite allP => x /=; rewrite mapP => He; elim He;smt(W256.size_w2bits).
-rewrite (nth_map W256.zero []); 1: smt(Array25.size_to_list).
-by rewrite nth_mkseq /#.
-qed.
-*)
-
-op sliceget256_64_25 (arr: W64.t Array25.t) (offset: int) : W256.t = 
- if 8 %| offset
- then  WArray200.get256_direct (WArray200.init64 (fun (i_0 : int) => arr.[i_0])) (offset %/ 8)
- else W256.bits2w (take 256 (drop offset (flatten (map W64.w2bits (to_list arr))))).
-
-(*
-bind op [W64.t & W256.t & Array25.t] sliceget256_64_25 "asliceget".
-realize bvaslicegetP.
-move => /= arr offset; rewrite /sliceget256_64_25 /= => H k kb. 
-case (8 %| offset) => /= *; last by smt(W256.get_bits2w).
-rewrite /get256_direct pack32E initiE 1:/# /= initiE 1:/# /= initiE 1:/# /= bits8E initiE 1:/# /=.
-rewrite nth_take 1,2:/# nth_drop 1,2:/#.
-rewrite (BitEncoding.BitChunking.nth_flatten false 64 _). 
- by rewrite allP => x /=; rewrite mapP => He; elim He;smt(W64.size_w2bits).
-rewrite (nth_map W64.zero []); 1: smt(Array25.size_to_list).
-by rewrite nth_mkseq /#.
-qed.
-*)
-
-op sliceset64_256_25 (arr: W256.t Array25.t) (offset: int) (bv: W64.t) : W256.t Array25.t =
- if 8 %| offset
- then Array25.init 
-       (fun i =>
-        WArray800.get256
-         (WArray800.set64_direct
-           (WArray800.init256 (fun j => arr.[j]))
-           (offset %/ 8)
-           bv)
-         i)
- else Array25.of_list
-       witness
-       (map W256.bits2w
-            (chunk 256
-                   (take offset (flatten (map W256.w2bits (to_list arr)))
-                     ++ w2bits bv ++
-                     drop (offset+64) (flatten (map W256.w2bits (to_list arr)))))).
-
-lemma size_flatten_W256_w2bits (a : W256.t list) :
-  (size (flatten (map W256.w2bits (a))))  =  256 * size a.
-proof.
-rewrite (size_flatten' 256).
- by move=> l /mapP [x [Hx ->]]; rewrite W256.size_w2bits.
-by rewrite size_map.
-qed.
-
-(*
-bind op [W256.t & W64.t & Array25.t] sliceset64_256_25 "asliceset".
-realize bvaslicesetP.
-move => arr offset bv H /= k kb; rewrite /sliceset64_256_25 /=.
-case (8 %| offset) => /= *; last first.
-+ rewrite of_listK; 1: by rewrite size_map size_chunk 1:// !size_cat size_take;
-      by smt(size_take size_drop  W256.size_w2bits size_cat Array25.size_to_list size_flatten_W256_w2bits size_ge0). 
-  rewrite -(map_comp W256.w2bits W256.bits2w) /(\o). 
-  have := eq_in_map ((fun (x : bool list) => w2bits ((bits2w x))%W256)) idfun (chunk 256
-        (take offset (flatten (map W256.w2bits (to_list arr))) ++ w2bits bv ++
-         drop (offset + 64) (flatten (map W256.w2bits (to_list arr))))).
-  rewrite iffE => [#] -> * /=; 1: by smt(in_chunk_size W256.bits2wK).
-  rewrite map_id /= chunkK 1://;1: by rewrite !size_cat size_take;
-    by smt(size_take size_drop  W256.size_w2bits size_cat Array25.size_to_list size_flatten_W256_w2bits size_ge0). 
-  by rewrite !nth_cat !size_cat /=;
-     smt(nth_take nth_drop size_take size_drop  W256.size_w2bits size_cat Array25.size_to_list size_flatten_W256_w2bits size_ge0). 
-rewrite (nth_flatten _ 256); 1: by rewrite allP => i;rewrite mapP => He; elim He;smt(W256.size_w2bits).
-rewrite (nth_map W256.zero []); 1: smt(Array25.size_to_list).
-rewrite nth_mkseq 1:/# /= initiE 1:/# /= get256E pack32E initiE 1:/# /= initiE 1:/# /= /set64_direct.
-rewrite initiE 1:/# /=.
-case (offset <= k && k < offset + 64) => *; 1: by 
-  rewrite ifT 1:/#  get_bits8 /= 1,2:/# initiE // initiE //.
-rewrite ifF 1:/# initiE 1:/# /=.
-rewrite (nth_flatten _ 256); 1: by rewrite allP => i;rewrite mapP => He; elim He;smt(W256.size_w2bits).
-rewrite (nth_map W256.zero []); 1: smt(Array25.size_to_list).
-rewrite nth_mkseq 1:/# /= bits8E /= initiE /# /=.
-qed.
-*)
-
-op sliceset256_64_25 (arr: W64.t Array25.t) (offset: int) (bv: W256.t) : W64.t Array25.t =
- if 8 %| offset
- then Array25.init 
-       (fun i =>
-        WArray200.get64
-         (WArray200.set256_direct
-           (WArray200.init64 (fun j => arr.[j]))
-           (offset %/ 8)
-           bv)
-         i)
- else Array25.of_list
-       witness
-       (map W64.bits2w
-            (chunk 64
-                   (take offset (flatten (map W64.w2bits (to_list arr)))
-                     ++ w2bits bv ++
-                     drop (offset+256) (flatten (map W64.w2bits (to_list arr)))))).
-
-lemma size_flatten_W64_w2bits (a : W64.t list) :
-  (size (flatten (map W64.w2bits (a))))  =  64 * size a.
-proof.
-rewrite (size_flatten' 64).
- by move=> l /mapP [x [Hx ->]]; rewrite W64.size_w2bits.
-by rewrite size_map.
-qed.
-
-(*
-bind op [W64.t & W256.t & Array25.t] sliceset256_64_25 "asliceset".
-realize bvaslicesetP. 
-move => arr offset bv H /= k kb; rewrite /sliceset256_64_25 /=.
-case (8 %| offset) => /= *; last first.
-+ rewrite of_listK; 1: by rewrite size_map size_chunk 1:// !size_cat size_take;
-      by smt(size_take size_drop  W64.size_w2bits size_cat Array25.size_to_list size_flatten_W64_w2bits size_ge0). 
-  rewrite -(map_comp W64.w2bits W64.bits2w) /(\o). 
-  have := eq_in_map ((fun (x : bool list) => w2bits ((bits2w x))%W64)) idfun (chunk 64
-        (take offset (flatten (map W64.w2bits (to_list arr))) ++ w2bits bv ++
-         drop (offset + 256) (flatten (map W64.w2bits (to_list arr))))).
-  rewrite iffE => [#] -> * /=; 1: by smt(in_chunk_size W64.bits2wK).
-  rewrite map_id /= chunkK 1://;1: by rewrite !size_cat size_take;
-    by smt(size_take size_drop  W64.size_w2bits size_cat Array25.size_to_list size_flatten_W64_w2bits size_ge0). 
-  by rewrite !nth_cat !size_cat /=;
-     smt(nth_take nth_drop size_take size_drop  W64.size_w2bits size_cat Array25.size_to_list size_flatten_W64_w2bits size_ge0). 
-rewrite (nth_flatten _ 64); 1: by rewrite allP => i;rewrite mapP => He; elim He;smt(W64.size_w2bits).
-rewrite (nth_map W64.zero []); 1: smt(Array25.size_to_list).
-rewrite nth_mkseq 1:/# /= initiE 1:/# /= get64E pack8E initiE 1:/# /= initiE 1:/# /= /set256_direct.
-rewrite initiE 1:/# /=.
-case (offset <= k && k < offset + 256) => *; 1: by 
-  rewrite ifT 1:/#  get_bits8 /= 1,2:/# initiE // initiE //.
-rewrite ifF 1:/# initiE 1:/# /=.
-rewrite (nth_flatten _ 64); 1: by rewrite allP => i;rewrite mapP => He; elim He;smt(W64.size_w2bits).
-rewrite (nth_map W64.zero []); 1: smt(Array25.size_to_list).
-rewrite nth_mkseq 1:/# /= bits8E /= initiE /# /=.
-qed.
-*)
 
 (** Packed 4x-state *)
 
 type state4x = W256.t Array25.t.
 
-(*
-abbrev st4x_get (a: state4x) (k: int): state =
- init_25_64 (fun i => u256_bits64 a.[i] k).
-*)
-op (*abbrev*) st4x_get a k=
+op st4x_get a k=
  init_25_64 (fun i => sliceget64_256_25 a (8*(4*i+k)*8)).
 
 
@@ -222,9 +68,7 @@ rewrite bits64iE // initiE //= initiE 1:/# /= initiE 1:/# /= bits8E initiE 1:/# 
 by congr; smt().
 qed.
 
-op init_25_256 (f : int -> W256.t) : W256.t Array25.t = Array25.init f.
-
-op (*abbrev*) st4x_pack (sts: state*state*state*state): state4x =
+op st4x_pack (sts: state*state*state*state): state4x =
  init_25_256 (fun i => u256_pack4 sts.`1.[i] sts.`2.[i] sts.`3.[i] sts.`4.[i]).
 
 lemma st4x_packiE (sts: state*state*state*state) i:
@@ -260,7 +104,7 @@ congr;
      rewrite st4x_getiE //= initiE //= u256_pack4E pack4bE //).
 qed.
 
-op (*abbrev*) st4x_map (f:W64.t Array25.t->W64.t Array25.t) (st4x:W256.t Array25.t): W256.t Array25.t =
+op st4x_map (f:W64.t Array25.t->W64.t Array25.t) (st4x:W256.t Array25.t): W256.t Array25.t =
  st4x_pack (f (st4x_get st4x 0), f (st4x_get st4x 1), f (st4x_get st4x 2), f (st4x_get st4x 3)).
 
 lemma st4x_mapE (f: state->state) (st4x: state4x):
@@ -271,121 +115,14 @@ apply Array25.ext_eq => i Hi.
 by rewrite initiE //= st4x_packiE. 
 qed.
 
-(*op st4x_match (st4x: state4x) (st0 st1 st2 st3: state) =
- st4x = st4x_pack (st0,st1,st2,st3).
-*)
-op (*abbrev*) st4x_match st4x sts = (st4x = st4x_pack sts).
-
-
-(*
-lemma a25bits64iE x k i:
- 0 <= i < 25 =>
- (x \a25bits64 k).[i] = x.[i] \bits64 k.
-proof. by move=> Hi; rewrite mapiE //. qed.
-
-lemma a24bits64iE x k i:
- 0 <= i < 24 =>
- (x \a24bits64 k).[i] = x.[i] \bits64 k.
-proof. by move=> Hi; rewrite mapiE //. qed.
-
-lemma a5bits64iE x k i:
- 0 <= i < 5 =>
- (x \a5bits64 k).[i] = x.[i] \bits64 k.
-proof. by move=> Hi; rewrite mapiE //. qed.
-
-lemma a25unpack4K s4:
- a25pack4 (a25unpack4 s4) = s4.
-proof.
-rewrite /a25pack4 /a25unpack4.
-apply Array25.ext_eq => i Hi; rewrite initiE //=.
-rewrite -iotaredE /= !a25bits64iE //=.
-rewrite -{5}(unpack64K s4.[i]); congr.
-by rewrite unpack64E init_of_list -iotaredE /=. 
-qed.
-
-lemma a25pack4_bits64 k (stl: state list):
- 0 <= k < 4 =>
- a25pack4 stl \a25bits64 k = nth st0 stl k.
-proof.
-move=> Hk; apply Array25.ext_eq => i Hi.
-rewrite mapiE //= initiE //= pack4bE //=.
-rewrite of_listE initiE //=.
-case: (k < size stl) => E.
- by rewrite (nth_map st0) 1:/#.
-rewrite !nth_out; first 2 by smt(size_map).
-by rewrite createiE.
-qed.
-
-op a5pack4 (l: (W64.t Array5.t) list): W256.t Array5.t =
- Array5.init (fun i => pack4 (map (fun (x: W64.t Array5.t) => x.[i]) l)).
-
-lemma a25pack4_eq stl st4x:
- a25pack4 stl = st4x
- <=>
- all (fun k=>st4x \a25bits64 k = nth st0 stl k) (iota_ 0 4).
-proof.
-split.
- move => <-; apply/List.allP => k. 
- rewrite mem_iota => Hk /=; apply a25pack4_bits64; smt().
-move=> /List.allP H.
-apply Array25.ext_eq => i Hi.
-rewrite initiE //=.
-rewrite -(unpack64K st4x.[i]); congr.
-apply W4u64.Pack.ext_eq => k Hk.
-rewrite of_listE unpack64E !initiE //=.
-rewrite -a25bits64iE // H; first smt(mem_iota).
-case: (k < size stl) => E.
- by rewrite (nth_map st0) 1:/#.
-rewrite !nth_out; first 2 by smt(size_map).
-by rewrite createiE.
-qed.
-
-lemma a5bits64_set (c: W256.t Array5.t) x y i:
- 0 <= i < 4 =>
- 0 <= x < 5 =>
- c.[x <- y] \a5bits64 i
- = (c \a5bits64 i).[x <- y \bits64 i].
-proof.
-move=> Hi Hx; apply Array5.ext_eq => j Hj.
-rewrite a5bits64iE 1:// !get_setE 1..2:/#.
-case: (j=x) => E //.
-by rewrite a5bits64iE.
-qed.
-
-lemma xorw_bits64 (w1 w2: W256.t) k:
- 0 <= k < 4 =>
- w1 `^` w2 \bits64 k = (w1 \bits64 k) `^` (w2 \bits64 k).
-proof.
-move=> Hk; rewrite -{1}(unpack64K w1) -{1}(unpack64K w2). 
-by rewrite xorb4u64E pack4bE // map2iE // !unpack64E !initiE.
-qed.
-
-
-op map_state4x (f:state->state) (st:state4x): state4x =
- a25pack4 (map f (a25unpack4 st)).
-
-lemma map_state4x_a25bits64 f st k:
- 0 <= k < 4 =>
- (map_state4x f st) \a25bits64 k = f (st \a25bits64 k).
-proof.
-move=> Hk.
-rewrite /map_state4x /a25unpack4 -map_comp /(\o) /= a25pack4_bits64 1:// -iotaredE.
-have: k \in iotared 0 4 by smt(mem_iota).
-by move: {Hk} k ; apply/List.allP.
-qed.
-
-*)
-(******************)
+op st4x_match st4x sts = (st4x = st4x_pack sts).
 
 
 (******************************************************************************
    
 ******************************************************************************)
 
-from CryptoSpecs require import Keccak1600_Spec.
 import BitEncoding BitChunking.
-from JazzEC require import Array25 WArray200.
-
 
 
 op keccak_f1600_x4 = st4x_map keccak_f1600_op.
