proof/amd64/avx2/Keccakf1600_avx2x4.ec
@@ -9,10 +9,11 @@ require import Keccakf1600_ref.
 require import Keccak1600_ref.
 require import Keccak1600_avx2x4.
 
-from JazzEC require import Keccak1600_Jazz.
-from JazzEC require import Array5 Array25.
+require import Keccak_bindings.
 
-from JazzEC require import WArray200 WArray800.
+from JazzEC require import Keccak1600_Jazz.
+
+from JazzEC require import Array100 WArray200 WArray800.
 
 op st4x_to_4st (st4x: state4x): state*state*state*state =
  ( init_25_64 (fun i => sliceget64_256_25 st4x ((200*0+8*i)*8))
@@ -21,89 +22,9 @@ op st4x_to_4st (st4x: state4x): state*state*state*state =
  , init_25_64 (fun i => sliceget64_256_25 st4x ((200*3+8*i)*8))
  ).
 
-from JazzEC require import Array100.
- 
-bind array Array25."_.[_]" Array25."_.[_<-_]" Array25.to_list Array25.of_list Array25.t 25.
-realize gt0_size by done.
-realize tolistP by done.
-realize get_setP by smt(Array25.get_setE). 
-realize eqP by smt(Array25.tP).
-realize get_out by smt(Array25.get_out).
-
-(*
-op init_25_64 (f: int -> W64.t) = Array25.init f.
-*)
-bind op [W64.t & Array25.t] init_25_64 "ainit".
-realize bvainitP.
-proof.
-rewrite /init_25_64 => f.
-rewrite BVA_Top_Array25_Array25_t.tolistP.
-apply eq_in_mkseq => i i_bnd;
-smt(Array25.initE).
-qed.
-bind op [W256.t & Array25.t] init_25_256 "ainit".
-realize bvainitP.
-proof.
-rewrite /init_25_256 => f.
-rewrite BVA_Top_Array25_Array25_t.tolistP.
-apply eq_in_mkseq => i i_bnd;
-smt(Array25.initE).
-qed.
 
 
-bind array Array100."_.[_]" Array100."_.[_<-_]" Array100.to_list Array100.of_list Array100.t 100.
-realize gt0_size by done.
-realize tolistP by done.
-realize get_setP by smt(Array100.get_setE). 
-realize eqP by smt(Array100.tP).
-realize get_out by smt(Array100.get_out).
-    
-op init_100_64 (f: int -> W64.t) = Array100.init f.
-
-bind op [W64.t & Array100.t] init_100_64 "ainit".
-realize bvainitP.
-proof.
-rewrite /init_100_64 => f.
-rewrite BVA_Top_Array100_Array100_t.tolistP.
-apply eq_in_mkseq => i i_bnd;
-smt(Array100.initE).
-qed.
-
-
-op sliceget256_64_100 (arr: W64.t Array100.t) (offset:int): W256.t =
- if 8 %| offset
- then WArray800.get256_direct
-       (WArray800.init64 (fun i => arr.[i]))
-       (offset %/ 8)
- else W256.bits2w (take 256 (drop offset (flatten (map W64.w2bits (to_list arr))))).
-
-bind op [W64.t & W256.t & Array100.t] sliceget256_64_100 "asliceget".
-realize le_size by done.       
-realize bvaslicegetP.
-move => /= arr offset; rewrite /sliceget256_64_100 /= => H k kb. 
-case (8 %| offset) => /= *; last by smt(W256.get_bits2w).
-rewrite /get256_direct pack32E initiE 1:/# /= initiE 1:/# /= initiE 1:/# /= bits8E initiE 1:/# /=.
-rewrite nth_take 1,2:/# nth_drop 1,2:/#.
-rewrite (BitEncoding.BitChunking.nth_flatten false 64 _). 
- by rewrite allP => x /=; rewrite mapP => He; elim He;smt(W64.size_w2bits).
-rewrite (nth_map W64.zero []); 1: smt(Array100.size_to_list).
-by rewrite nth_mkseq /#.
-qed.
-
-bind op [W256.t & W64.t & Array25.t] sliceget64_256_25 "asliceget".
-realize le_size by done.       
-realize bvaslicegetP.
-admit.
-qed.
-
-bind op [W64.t & W256.t & Array25.t] sliceget256_64_25 "asliceget".
-realize le_size by done.       
-realize bvaslicegetP.
-admit.
-qed.
-
-
-op (*abbrev*) st4x_from_4st (sts: state*state*state*state): state4x =
+op st4x_from_4st (sts: state*state*state*state): state4x =
  init_25_256
   (fun i =>
     sliceget256_64_100
@@ -121,7 +42,7 @@ lemma st4x_from_4stK sts:
 proof.
 move: sts => [st0 st1 st2 st3].
 rewrite /st4x_to_4st /=.
-do split;
+by do split;
  rewrite tP => i Hi;
  rewrite initiE //= /sliceget64_256_25 ifT 1:/# get64E;
  apply W64.ext_eq => k Hk;
@@ -132,7 +53,7 @@ do split;
  rewrite get256E pack32E /= bits8iE 1:/#;
  rewrite initiE 1:/# /= initiE 1:/# /=;
  rewrite initiE 1:/# /= initiE 1:/# /=;
- by rewrite !bits8iE /#.
+ rewrite !bits8iE /#. 
 qed.
 
 lemma st4x_from_4stK' st0 st1 st2 st3:
@@ -181,8 +102,6 @@ by rewrite -(st4x_from_4stK sts1) H st4x_from_4stK.
 qed.
 
 lemma st4x_from_4st_inj' (st0a st1a st2a st3a st0b st1b st2b st3b: state):
- (* st4x_from_4st (st0a,st1a,st2a,st3a)
-    = st4x_from_4st (st0b,st1b,st2b,st3b) => *)
  init_25_256
   (fun (i : int) =>
      sliceget256_64_100
@@ -211,26 +130,13 @@ qed.
 
 require import Avx2_extra.
 
-(*
-abbrev st4x_pack' (st0 st1 st2 st3: state) =
- init_25_256
-    (fun (i : int) => u256_pack4 st0.[i] st1.[i] st2.[i] st3.[i]).
-*)
 op st4x_pack_spec (sts: state4x): state4x =
  st4x_pack (st4x_to_4st sts).
-(*
-abbrev st4x_pack4 (sts: state*state*state*state) =
- st4x_pack' sts.`1 sts.`2 sts.`3 sts.`4.
 
-op st4x_pack_spec' (sts: state4x): state4x =
- st4x_pack4 (st4x_to_4st sts).
-*)
 op st4x_unpack_spec (st4x: state4x) =
  st4x_from_4st (st4x_unpack st4x).
 
 op st4x_inv (_: state4x) = true.
-
-from CryptoSpecs require import Bindings.
 
 lemma st4x_get_pack0' (st0 st1 st2 st3: state):
  init_25_64
@@ -250,7 +156,7 @@ lemma st4x_get_pack1' (st0 st1 st2 st3: state):
   1
  = st1.
 proof.
-circuit.
+by circuit.
 qed.
 
 lemma st4x_get_pack2' (st0 st1 st2 st3: state):
@@ -259,7 +165,7 @@ lemma st4x_get_pack2' (st0 st1 st2 st3: state):
   2
  = st2.
 proof.
-circuit.
+by circuit.
 qed.
 
 lemma st4x_get_pack3' (st0 st1 st2 st3: state):
@@ -268,49 +174,35 @@ lemma st4x_get_pack3' (st0 st1 st2 st3: state):
   3
  = st3.
 proof.
-circuit.
+by circuit.
 qed.
 
 lemma st4x_get_pack0 sts:
  st4x_get (st4x_pack sts) 0 = sts.`1.
 proof.
 move: sts => [st0 st1 st2 st3] /=.
-circuit.
-(*
-rewrite tP => i Hi.
-rewrite initiE //= /init_25_256 /sliceget64_256_25 ifT 1:/#.
-rewrite (:8 * (4 * i) * 8 %/ 8=8*(4*i)) 1:/#.
-rewrite get64E pack8E.
-apply W64.ext_eq => k Hk.
-rewrite initiE //= initiE 1:/# /=.
-rewrite initiE 1:/# /= initiE 1:/# /=.
-rewrite /u256_pack4 /concat_2u128 /concat_2u64 pack2E.
-rewrite bits8iE 1:/# W256.initiE 1:/# /=.
-rewrite !pack2E /= get_of_list 1:/# /=.
-rewrite ifT 1:/#.
-by rewrite W128.initiE 1:/# /= get_of_list 1:/# /= ifT /#.
-*)
+by circuit.
 qed.
 
 lemma st4x_get_pack1 sts:
  st4x_get (st4x_pack sts) 1 = sts.`2.
 proof.
 move: sts => [st0 st1 st2 st3] /=.
-circuit.
+by circuit.
 qed.
 
 lemma st4x_get_pack2 sts:
  st4x_get (st4x_pack sts) 2 = sts.`3.
 proof.
 move: sts => [st0 st1 st2 st3] /=.
-circuit.
+by circuit.
 qed.
 
 lemma st4x_get_pack3 sts:
  st4x_get (st4x_pack sts) 3 = sts.`4.
 proof.
 move: sts => [st0 st1 st2 st3] /=.
-circuit.
+by circuit.
 qed.
 
 
@@ -322,47 +214,10 @@ rewrite /st4x_unpack.
 by rewrite st4x_get_pack0 st4x_get_pack1 st4x_get_pack2 st4x_get_pack3.
 qed.
 
-(*
-lemma st4x_packK' st0 st1 st2 st3:
- st4x_unpack (st4x_pack' st0 st1 st2 st3) = (st0,st1,st2,st3).
-proof.
-rewrite /st4x_unpack.
-by rewrite st4x_get_pack0' st4x_get_pack1' st4x_get_pack2' st4x_get_pack3'.
-qed.
-*)
-(*
-lemma st4x_pack_inj sts1 sts2:
- st4x_pack sts1 = st4x_pack sts2
- => sts1 = sts2.
-proof.
-move=> H.
-by rewrite -{1}st4x_packK H st4x_packK.
-qed.
-*)
-
 lemma st4x_unpackK_ALT st4x:
  st4x_pack (st4x_unpack st4x) = st4x.
 proof.
-circuit.
-(*
-rewrite /st4x_unpack /st4x_pack tP => i Hi.
-rewrite st4x_packiE //; iota.
-rewrite !st4x_getiE //.
-rewrite /u256_pack4 /concat_2u128 /concat_2u64 pack2E.
-apply W256.ext_eq => k Hk.
-rewrite initiE 1:/# /= get_of_list 1:/# /=.
-case: (k < 128) => C1.
- rewrite ifT 1:/# pack2E.
- rewrite initiE 1:/# /= get_of_list 1:/# /=.
- case: (k < 64) => C2.
-  by rewrite ifT 1:/# bits64iE /#.
- by rewrite ifF 1:/# ifT 1:/# bits64iE /#.
-rewrite ifF 1:/# pack2E ifT 1:/#.
-rewrite initiE 1:/# /= get_of_list 1:/# /=.
-case: (k < 192) => C2.
- by rewrite ifT 1:/# bits64iE /#.
-by rewrite ifF 1:/# ifT 1:/# bits64iE /#.
-*)
+by circuit.
 qed.
 
 lemma st4x_unpack_inj st4x1 st4x2:
@@ -372,183 +227,6 @@ proof.
 move=> H.
 by rewrite -{1}st4x_unpackK H st4x_unpackK.
 qed.
-
-import BitEncoding BitChunking.
-lemma chunk1 ['a] n (l: 'a list):
- size l = n =>
- n <> 0 =>
- chunk n l = [l].
-proof.
-rewrite /chunk.
-move=> Hn H0.
-by rewrite Hn divzz H0 b2i1 mkseq1 /= drop0 -Hn take_size.
-qed.
-
-abbrev st_to_bv (st: state) =
- flatten (map W64.w2bits (to_list st)).
-
-abbrev st_from_bv (l: bool list) =
- Array25.of_list W64.zero (map W64.bits2w (chunk 64 l)).
-
-abbrev st4x_to_bv (st4x: state4x) =
- flatten (map W256.w2bits (to_list st4x)).
-
-abbrev st4x_from_bv (l: bool list) =
- Array25.of_list W256.zero (map W256.bits2w (chunk 256 l)).
-
-lemma size_st_to_bv st:
- size (st_to_bv st) = 1600.
-proof.
-rewrite (size_flatten' 64).
- move=> x /mapP [y [Hy ->]].
- exact W64.size_w2bits.
-by rewrite size_map size_to_list.
-qed.
-
-lemma size_st4x_to_bv st4x:
- size (st4x_to_bv st4x) = 6400.
-proof.
-rewrite (size_flatten' 256).
- move=> x /mapP [y [Hy ->]].
- exact W256.size_w2bits.
-by rewrite size_map size_to_list.
-qed.
-
-lemma st_to_bvK st:
- st_from_bv (st_to_bv st)
- = st.
-proof.
-rewrite flattenK //.
- move=> l /mapP [y [Hy ->]].
- by rewrite size_w2bits.
-rewrite -map_comp /(\o) id_map //=.
-by rewrite to_listK.
-qed.
-
-lemma st4x_to_bvK st4x:
- st4x_from_bv (st4x_to_bv st4x)
- = st4x.
-proof.
-rewrite flattenK //.
- move=> l /mapP [y [Hy ->]].
- by rewrite size_w2bits.
-rewrite -map_comp /(\o) id_map //=.
-by rewrite to_listK.
-qed.
-
-lemma st_from_bvK l:
- size l = 1600 =>
- st_to_bv (st_from_bv l)
- = l.
-proof.
-move=> Hl.
-rewrite of_listK.
- by rewrite size_map size_chunk // Hl /#.
-rewrite -map_comp /(\o).
-have ->:
- map (fun x => w2bits (W64.bits2w x)) (chunk 64 l)
- = map idfun (chunk 64 l).
- apply eq_in_map => //=.
- by move=> x Hx /=; rewrite /idfun bits2wK; smt(in_chunk_size).
-by rewrite map_id chunkK /#.
-qed.
-
-lemma st4x_from_bvK l:
- size l = 6400 =>
- st4x_to_bv (st4x_from_bv l)
- = l.
-proof.
-move=> Hl.
-rewrite of_listK.
- by rewrite size_map size_chunk // Hl /#.
-rewrite -map_comp /(\o).
-have ->:
- map (fun x => w2bits (W256.bits2w x)) (chunk 256 l)
- = map idfun (chunk 256 l).
- apply eq_in_map => //=.
- by move=> x Hx /=; rewrite /idfun W256.bits2wK; smt(in_chunk_size).
-by rewrite map_id chunkK /#.
-qed.
-
-lemma st4x_from_bv_inj l1 l2:
- size l1 = 6400 =>
- size l2 = 6400 =>
- st4x_from_bv l1 = st4x_from_bv l2
- => l1 = l2.
-proof.
-move=> H1 H2 H.
-by rewrite -{1}st4x_from_bvK // H st4x_from_bvK //.
-qed.
-
-lemma st4x_to_bv_from_4st st0 st1 st2 st3:
-(* st4x_to_bv (st4x_from_4st (st0,st1,st2,st3)) *)
- st4x_to_bv
-  (init_25_256
-    (fun (i : int) =>
-      sliceget256_64_100
-       (init_100_64
-         (fun (j : int) =>
-            if j < 25 then st0.[j]
-            else
-             if j < 50 then st1.[j - 25]
-             else if j < 75 then st2.[j - 50] else st3.[j - 75]))
-       (32 * i * 8)))
- = flatten [ st_to_bv st0
-           ; st_to_bv st1
-           ; st_to_bv st2
-           ; st_to_bv st3 ].
-proof.
-simplify.
-apply (eq_from_nth false).
- rewrite size_st4x_to_bv (size_flatten' 1600) //.
- by move=> x /= [->|[->|[->|->]]]; rewrite size_st_to_bv.
-move=> i; rewrite size_st4x_to_bv => Hi.
-rewrite (nth_flatten false 256).
- by rewrite allP => x /mapP [y [Hy ->]] /=.
-rewrite (nth_map witness).
- by rewrite size_to_list /#.
-rewrite get_to_list initiE 1:/# /= /sliceget256_64_100 ifT 1:/#.
-rewrite get256E pack32E initiE 1:/# /= initiE 1:/# /=.
-rewrite initiE 1:/# /= initiE 1:/# /=.
-rewrite (nth_flatten false 1600).
- by rewrite allP => x /= [->|[->|[->|->]]]; rewrite size_st_to_bv.
-case: (i < 1600) => C1.
- rewrite (:i %/ 1600=0) 1:/# /=.
- rewrite ifT 1:/# bits8E initiE 1:/# /=.
- rewrite (nth_flatten false 64).
-  by rewrite allP => x /mapP [y [Hy ->]].
- rewrite (nth_map witness).
-  by rewrite size_to_list /#.
- by rewrite get_to_list get_w2bits /#.
-case: (i < 3200) => C2.
- rewrite (:i %/ 1600=1) 1:/# /=.
- rewrite ifF 1:/# ifT 1:/# bits8E initiE 1:/# /=.
- rewrite (nth_flatten false 64).
-  by rewrite allP => x /mapP [y [Hy ->]].
- rewrite (nth_map witness).
-  by rewrite size_to_list /#.
- by rewrite get_to_list get_w2bits /#.
-case: (i < 4800) => C3.
- rewrite (:i %/ 1600=2) 1:/# /=.
- rewrite ifF 1:/# ifF 1:/# ifT 1:/# bits8E initiE 1:/# /=.
- rewrite (nth_flatten false 64).
-  by rewrite allP => x /mapP [y [Hy ->]].
- rewrite (nth_map witness).
-  by rewrite size_to_list /#.
- by rewrite get_to_list get_w2bits /#.
-rewrite (:i %/ 1600=3) 1:/# /=.
-rewrite ifF 1:/# ifF 1:/# ifF 1:/# bits8E initiE 1:/# /=.
-rewrite (nth_flatten false 64).
- by rewrite allP => x /mapP [y [Hy ->]].
-rewrite (nth_map witness).
- by rewrite size_to_list /#.
-by rewrite get_to_list get_w2bits /#.
-qed.
-
-bind op [W256.t & W64.t & Array25.t] sliceset64_256_25 "asliceset".
-realize le_size by done.
-realize bvaslicesetP.
-admitted. 
 
 
 hoare st4x_pack_h _st0 _st1 _st2 _st3:
@@ -576,7 +254,7 @@ proc change 63: { st4x <- sliceset64_256_25 st4x (8*(4 * 24 + 3)*8) t3; };
  1: by auto => /#.
 inline*; simplify.
 swap 127 8; wp 134.
-circuit.
+by circuit.
 qed.
 
 lemma st4x_pack_ll: islossless M.__st4x_pack.
@@ -597,41 +275,27 @@ hoare st4x_unpack_h _st4x:
  ==> res = st4x_unpack _st4x.
 proof.
 proc; simplify.
-admit(*
-proc change ^while.6: (sliceset256_64_25 st0 (4*8*i*8) x0);
+proc change ^while.6: { st0 <- sliceset256_64_25 st0 (4*8*i*8) x0; };
  1: by auto => /#.
-proc change ^while.7: (sliceset256_64_25 st1 (4*8*i*8) x1);
+proc change ^while.7: { st1 <- sliceset256_64_25 st1 (4*8*i*8) x1; };
  1: by auto => /#.
-proc change ^while.8: (sliceset256_64_25 st2 (4*8*i*8) x2);
+proc change ^while.8: { st2 <- sliceset256_64_25 st2 (4*8*i*8) x2; };
  1: by auto => /#.
-proc change ^while.9: (sliceset256_64_25 st3 (4*8*i*8) x3);
+proc change ^while.9: { st3 <- sliceset256_64_25 st3 (4*8*i*8) x3; };
  1: by auto => /#.
-proc change 3: (sliceget64_256_25 st4x (8*(4*24)*8));
+proc change 3: { t0 <- sliceget64_256_25 st4x (8*(4*24)*8); };
  1: by auto => /#.
-proc change 4: (sliceget64_256_25 st4x (8*(4*24+1)*8));
+proc change 4: { t1 <- sliceget64_256_25 st4x (8*(4*24+1)*8); };
  1: by auto => /#.
-proc change 5: (sliceget64_256_25 st4x (8*(4*24+2)*8));
+proc change 5: { t2 <- sliceget64_256_25 st4x (8*(4*24+2)*8); };
  1: by auto => /#.
-proc change 6: (sliceget64_256_25 st4x (8*(4*24+3)*8));
+proc change 6: { t3 <- sliceget64_256_25 st4x (8*(4*24+3)*8); };
  1: by auto => /#.
 unroll for 2.
 swap 55 8.
 wp 62.
 inline*.
-bdep 6400 6400
-     [_st4x] [st4x] [st0;st1;st2;st3]
-     st4x_unpack_spec
-     st4x_inv.
-+ by move=> &m /> *; rewrite all_predT.
-move=> &m /> st0 st1 st2 st3 /=.
-rewrite flatten1 chunk1 1:size_st4x_to_bv //=.
-rewrite (chunk1 6400) //=.
- rewrite (size_flatten' 1600) //.
- by move=> x /= [->|[->|[->|->]]]; rewrite size_st_to_bv.
-rewrite /st4x_unpack_spec /st4x_unpack.
-rewrite !st4x_to_bvK -st4x_to_bv_from_4st st4x_to_bvK.
-by move=> /st4x_from_4st_inj' />.
-*).
+by circuit.
 qed.
 
 lemma st4x_unpack_ll: islossless M.__st4x_unpack.
@@ -686,7 +350,7 @@ hoare keccak_pround_unpacked_h _st4x:
      /\ (st4x_to_4st res).`4 = keccak_pround_op (st4x_to_4st _st4x).`4.
 proof.
 proc; inline*; simplify.
-circuit.
+by circuit.
 qed.
 
 lemma keccakf1600_4x_pround_ll: islossless M._keccakf1600_4x_pround.
@@ -713,17 +377,9 @@ equiv keccak_pround_avx2x4_eq:
    /\ r8{1} = rOL8 /\ r56{1} = rOL56
  ==> ={res}.
 proof.
-(* ...não consigo usar o bdepeq!!! (obs: deverá ser da inicialização de (r8,r56){1}...)
-proc; inline*; simplify.
-bdepeq 6400 [a] [st4x1] {6400: [e ~ st4x2]} st4x_inv.
-*)
-proc; inline*; simplify.
-wp 261 258.
-conseq (_: _ ==> e{1}=e{2}).
- move=> &1 &2 /> e.
- by rewrite st4x_from_4stK st4x_unpackK.
-sim; auto => /> &m.
-by rewrite /st4x_pack_spec /st4x_unpack_spec st4x_from_4stK st4x_unpackK.
+proc.
+inline*.
+by circuit.
 qed.
 
 op st4x_keccak_pround =
@@ -783,10 +439,7 @@ proof.
 proc; simplify.
 (* não consegue lidar com isto... (grande demais?)*)
 abort. (*
-bdep 6400 6400
- [_st4x] [a] [e]
- st4x_keccak_pround st4x_inv.
-admitted.
+circuit.
 *)
 
 from JazzEC require import Array24.
@@ -796,7 +449,7 @@ abbrev keccak_round_i i st =
 abbrev st_keccak_iota rc (st:state) =
  st.[0 <- st.[0] `^` rc].
 abbrev st4x_keccak_iota rc (st4x:state4x) =
- st4x.[0 <- st4x.[0] `^` VPBROADCAST_4u64 rc].
+ st4x.[0 <- VPBROADCAST_4u64 rc `^` st4x.[0]].
 
 
 lemma VPBROADCAST_4u64_bits64 w k:
@@ -806,9 +459,7 @@ proof.
 move=> Hk; have: k\in iota_ 0 4 by smt(mem_iota).
 move: {Hk} k; apply/List.allP.
 rewrite -iotaredE /=.
-admit (*
-by bdep solve.
-*).
+by circuit.
 qed.
 
 lemma sliceget64_256_25E k i st4x:
@@ -823,7 +474,6 @@ apply W64.ext_eq => b Hb.
 rewrite !initiE //= pack8E initiE //= initiE 1:/# /= initiE 1:/# /=.
 by rewrite bits8iE 1:/# /#.
 qed.
-
 
 
 lemma st4x_keccak_iotaE rc st4x:
@@ -841,7 +491,7 @@ rewrite -iotaredE /=.
 case: (i=0) => Ei.
  rewrite (sliceget64_256_25E 0 0) // (sliceget64_256_25E 1 0) //.
  rewrite (sliceget64_256_25E 2 0) // (sliceget64_256_25E 3 0) //.
- by rewrite !xorb64E !VPBROADCAST_4u64_bits64 //.
+ by rewrite xorwC !xorb64E !VPBROADCAST_4u64_bits64 //.
 rewrite (sliceget64_256_25E 0 i) // (sliceget64_256_25E 1 i) //.
 by rewrite (sliceget64_256_25E 2 i) // (sliceget64_256_25E 3 i) //.
 qed.
@@ -914,29 +564,9 @@ while (0 <= c <= 24 /\ c %% 2 = 0 /\
  pose st2:= (st4x_get _ _).
  pose st3:= (st4x_get _ _).
  pose st4x1 := (st4x_pack _).
-admit (*
- pose st0:= (init_25_64 _).
- pose st1:= (init_25_64 _).
- pose st2:= (init_25_64 _).
- pose st3:= (init_25_64 _).
- pose st4x1 := (init_25_256 _).
- rewrite -st4x_keccak_roundP2 //=. 
- rewrite tP => i Hi.
- rewrite Array25.initiE // eq_sym Array25.initiE //=.
- pose sts:= ( keccak_round_i (to_uint c{m}) st0
-            , keccak_round_i (to_uint c{m}) st1
-            , keccak_round_i (to_uint c{m}) st2
-            , keccak_round_i (to_uint c{m}) st3 ).
- congr.
- + congr; congr; congr.
-   by rewrite /st4x1 (st4x_get_pack0 sts) /#.
- + congr; congr; congr. 
-   by rewrite /st4x1 (st4x_get_pack1 sts) /#.
- + congr; congr; congr. 
-   by rewrite /st4x1 (st4x_get_pack2 sts) /#.
- + congr; congr; congr. 
-   by rewrite /st4x1 (st4x_get_pack3 sts) /#.
-*).
+ move: (st4x_keccak_roundP2 rc_spec.[c{m}] rc_spec.[c{m} + 1] st4x1).
+ rewrite st4x_get_pack0 st4x_get_pack1 st4x_get_pack2 st4x_get_pack3 /=.
+ by move => -> /=.
 auto => |>; split.
  rewrite iota0 //= tP => i Hi.
  rewrite initiE //= (st4x_getiE _ 0) // !st4x_getiE //.
@@ -944,7 +574,7 @@ auto => |>; split.
  rewrite !bits64E.
  apply W256.ext_eq => k Hk.
  rewrite pack4wE // get_of_list 1:/#.
- smt(W64.initiE).
+ smt(W64.initiE). 
 by move=> c ???; have ->: c = 24; smt().
 qed.
 
